ModularEngine/src/LogicEngine.FStar.Wrapper/utilities.fs
@@ -11,11 +11,15 @@
 
 namespace Microsoft.Research.Dkal.LogicEngine.FStar.Wrapper
 
+open System.Collections.Generic
+
 open Microsoft.Research.Dkal.Interfaces
 open Microsoft.Research.Dkal.Substrate
+open Microsoft.Research.Dkal.LogicEngine.FStar.Deps
 
 module Utilities =
   type principal = string
+  type substitution = Dictionary<Types.var, Types.term>
 
   let _value_knowledge (_infostrate : IInfostrate option) =
     _infostrate.Value.Knowledge |> Seq.toList |>
@@ -33,3 +37,57 @@ module Utilities =
     SubstrateDispatcher.Solve q' s' |> Seq.toList |>
     List.map TranslationToFStar.FStarSubstitutionOfISubstitution
 
+  (* For CoreDKAL2 only *)
+  let substrateQueryTerm_Vars (s:Builders.substrateQueryTerm) : Prims.list<Types.var> =
+    Builders.PrimsListOfList (List.map TranslationToFStar.FStarVarOfIVar s.Vars)
+  let substrateUpdateTerm_Vars (s:Builders.substrateUpdateTerm) : Prims.list<Types.var> =
+    Builders.PrimsListOfList (List.map TranslationToFStar.FStarVarOfIVar s.Vars)
+  let substrateQueryTerm_boundVars (s:Builders.substrateQueryTerm) : Prims.list<Types.var> =
+    Builders.PrimsListOfList (List.map TranslationToFStar.FStarVarOfIVar s.BoundVars)
+  let substrateUpdateTerm_boundVars (s:Builders.substrateUpdateTerm)  : Prims.list<Types.var> =
+    Builders.PrimsListOfList (List.map TranslationToFStar.FStarVarOfIVar s.BoundVars)
+  (*let substrateQueryTerm_apply (s:Builders.substrateQueryTerm) (s2:ISubstitution) : ITerm = s.Apply s2
+  let substrateUpdateTerm_apply (s:Builders.substrateUpdateTerm) (s2:ISubstitution) : ITerm = s.Apply s2
+  let _substrateQueryTerm_unifyFrom (s:Builders.substrateQueryTerm) (s2:ISubstitution) (t:ITerm) : ISubstitution option = s.UnifyFrom s2 t
+  let _substrateUpdateTerm_unifyFrom (s:Builders.substrateUpdateTerm) (s2:ISubstitution) (t:ITerm) : ISubstitution option = s.UnifyFrom s2 t
+  *)
+
+  (* solution 1 (preferred but does not compile *)
+  let mkSubst (al:Prims.list<Types.var>) (bl:Prims.list<Types.term>) : substitution =
+    let res = new Dictionary<Types.var, Types.term>() in
+    List.iter2 (fun a b -> res.[a] <- b)
+      ((TypeHeaders.ListOfPrimsList.TyApp<Types.var>() 
+          :?> (Prims.list<Types.var> -> list<Types.var>)) al)
+      ((TypeHeaders.ListOfPrimsList.TyApp<Types.term>() 
+          :?> (Prims.list<Types.term> -> list<Types.term>)) bl);
+    res
+  (* solution 2 (but can only compile the subst.fst with --UNSAFE) *)
+  (*
+  let mkSubst_aux (al:list<Types.var>) (bl:list<Types.term>) : substitution =
+    let res = new Dictionary<Types.var, Types.term>() in
+    List.iter2 (fun a b -> res.[a] <- b) al bl;
+    res
+  *)
+  let substQuery (q:ISubstrateQueryTerm) (s:substitution) : ISubstrateQueryTerm =
+    q.Apply(TranslationFromFStar.ISubstitutionOfFStarSubstitution s)
+      :?> ISubstrateQueryTerm
+
+  let emptySubst (b:bool) : substitution = 
+    new Dictionary<Types.var, Types.term>()
+
+  let extendSubst (s:substitution) (x:Types.var) (t:Types.term) =
+      (* simple extension for now; does not replace x in all the images of s *)
+      let newSubst = new Dictionary<_, _>(s)
+      newSubst.[x] <- t
+      newSubst
+  
+  let extends (s2:substitution) (s1:substitution) : bool =
+    true (* TODO: dummy, need to get rid of it eventually *)
+
+  let lookupVar (s:substitution) (x:Types.var) : Prims.option<Types.term> = 
+    let found, ret = s.TryGetValue x in
+    (if found then Some(ret) else None)
+    |> Builders.PrimsOptionOfOption
+
+  let domain (s:substitution) : Prims.list<Types.var> =
+    [ for kvp in s -> kvp.Key ] |> Builders.PrimsListOfList
